Def. chg_end_acc and Thm. chg_enc_acc_sum_leng revised

examples/Crypto/RIPEMD/ripemd160Script.sml
@@ -1,8 +1,7 @@
 open HolKernel boolLib bossLib Parse
      listTheory rich_listTheory
-     arithmeticTheory logrootTheory
-     bitTheory wordsTheory
-     numposrepTheory byteTheory wordsLib
+     arithmeticTheory logrootTheory numposrepTheory
+     byteTheory wordsTheory wordsLib
      cv_stdTheory cv_transLib
      intLib
 
@@ -13,9 +12,9 @@ val _ = new_theory"ripemd160";
 
 (* auxiliary function used in chg_end_def *)
 Definition chg_end_acc_def:
-  chg_end_acc acc [] = acc ∧
-  chg_end_acc acc (b::bits) =
-  chg_end_acc (TAKE 8 (b::bits) ++ acc) (DROP 8 (b::bits))
+  chg_end_acc acc bits =
+  if NULL bits then acc
+  else chg_end_acc (TAKE 8 bits ++ acc) (DROP 8 bits)
 Termination
   WF_REL_TAC`measure (LENGTH o SND)` \\ Cases \\ rw[]
 End
@@ -23,13 +22,35 @@ End
 Theorem chg_end_acc_sum_leng:
   ∀acc bits. LENGTH $ chg_end_acc acc bits = LENGTH acc + LENGTH bits
 Proof
-  ho_match_mp_tac chg_end_acc_ind>>
-  rw[chg_end_acc_def, listTheory.LENGTH_TAKE_EQ]
+  Induct_on ‘LENGTH bits DIV 8’>>
+  rw[ADD1]
+  >-(
+    fs[dividesTheory.DIV_EQUAL_0]>>
+    Cases_on ‘NULL bits’>>
+    rw[Once chg_end_acc_def]
+    >-fs[NULL_LENGTH]
+    >-rw[DROP_LENGTH_TOO_LONG,Once chg_end_acc_def,LENGTH_TAKE_EQ])
+  >-(
+    Cases_on ‘NULL bits’
+    >-fs[NULL_LENGTH]
+    >-(
+      rw[Once chg_end_acc_def]>>
+      pop_assum kall_tac>>
+      last_x_assum $ qspec_then ‘DROP 8 bits’ assume_tac>>
+      ‘v = LENGTH (DROP 8 bits) DIV 8’ by (
+        simp[LENGTH_DROP]>>
+        ‘8 ≤ LENGTH bits’ by (
+          ‘LENGTH bits DIV 8 ≠ 0’ by simp[]>>
+          ‘0 < 8’ by simp[]>>
+          gvs[dividesTheory.DIV_EQUAL_0])>>
+        simp[dividesTheory.SUB_DIV])>>
+      fs[]>>
+      simp[LENGTH_TAKE_EQ]))
 QED
 
 (* change bits in little-endian to that in big-endian or vice versa, padding 0s to the left of bits when necessary to make the length of bits a multiple of 8 *)
 Definition chg_end_def:
-  chg_end (bits: num list) =
+  chg_end bits: num list =
   let
     l = LENGTH bits;
     n = l MOD 8;
@@ -41,14 +62,10 @@ End
 Theorem chg_end_length_multiple:
   divides 8 $ LENGTH (chg_end bits)
 Proof
-  simp[chg_end_def, chg_end_acc_sum_leng, dividesTheory.DIVIDES_MOD_0]>>
-  Cases_on ‘LENGTH bits MOD 8’
-  >-simp[Once $ GSYM MOD_PLUS]>>
+  simp[chg_end_def,chg_end_acc_sum_leng,dividesTheory.DIVIDES_MOD_0]>>
+  Cases_on ‘LENGTH bits MOD 8’>>
   simp[Once $ GSYM MOD_PLUS]>>
-  ‘SUC n < 8’ by (
-    pop_assum (SUBST1_TAC o GSYM)>>
-    simp[MOD_LESS])>>
-  simp[]
+  intLib.ARITH_TAC
 QED
 
 Theorem chg_end_length:
@@ -62,7 +79,7 @@ Definition pad_message_def:
   let
     l  = LENGTH bits;
     n  = (l + 1) MOD 512;
-    k  = if n <= 448 then 448 - n else 512 + 448 - n;
+    k  = if n ≤ 448 then 448 - n else 512 + 448 - n;
     lb = chg_end $ PAD_LEFT 0 64 (if l = 0 then [] else REVERSE $ n2l 2 l)
   in
     bits ++ (1 :: REPLICATE k 0) ++ lb
@@ -78,9 +95,9 @@ Proof
   ‘LENGTH (n2l 2 (LENGTH bits)) ≤ 64’ by (
     ‘LENGTH bits ≤ 2 ** 64 - 1’ by decide_tac>>
     Cases_on ‘LENGTH bits’>>
-    simp[numposrepTheory.LENGTH_n2l]>>
+    simp[LENGTH_n2l]>>
     ‘0 < SUC n’ by simp[]>>
-    drule_then assume_tac logrootTheory.LOG2_LE_MONO>>
+    drule_then assume_tac logrootTheory.LOG2_LE_MONO>> (*why not bitTheory?*)
     pop_assum $ drule_then assume_tac>>
     gvs[])>>
   rw[pad_message_def]>>
@@ -92,9 +109,12 @@ Proof
 QED
 
 Definition parse_block_def:
-  parse_block acc bits =
-  if NULL bits then REVERSE acc : word32 list
-  else parse_block ((word_from_bin_list $ REVERSE $ chg_end $ TAKE 32 bits)::acc) (DROP 32 bits)
+  parse_block acc bits: word32 list =
+  if NULL bits then REVERSE acc
+  else
+    parse_block
+      ((word_from_bin_list $ REVERSE $ chg_end $ TAKE 32 bits)::acc)
+      (DROP 32 bits)
 Termination
   WF_REL_TAC`measure (LENGTH o SND)` \\ Cases \\ rw[]
 End
@@ -102,28 +122,24 @@ End
 (* parse bits (assumed to have length that is a multiple of 512) into blocks, each of which is a schedule consisting of 16 words of 32 bits *)
 Definition parse_message_def:
   parse_message acc bits =
-  if NULL bits then REVERSE acc else
-  parse_message (parse_block [] (TAKE 512 bits) :: acc) (DROP 512 bits)
+  if NULL bits then REVERSE acc
+  else parse_message (parse_block [] (TAKE 512 bits) :: acc) (DROP 512 bits)
 Termination
   WF_REL_TAC`measure (LENGTH o SND)` \\ Cases \\ rw[]
 End
 
 val () = cv_auto_trans parse_message_def;
 
-
-
-
-(*** BEGIN ***)
-
 Theorem parse_block_size:
-  ∀n acc bits. LENGTH bits = 32 * n ⇒ LENGTH $ parse_block acc bits = LENGTH acc + n
+  ∀n acc bits.
+    LENGTH bits = 32 * n ⇒ LENGTH $ parse_block acc bits = LENGTH acc + n
 Proof
   Induct
   >-rw[Once parse_block_def]
   >-(
     rw[ADD1]>>
-    Cases_on ‘NULL bits’ (* to revise *)
-    >-fs[listTheory.NULL_LENGTH]
+    Cases_on ‘NULL bits’
+    >-fs[NULL_LENGTH]
     >-simp[Once parse_block_def])
 QED
 
@@ -138,20 +154,14 @@ Proof
   gvs[]>>
   last_x_assum irule>>
   CONJ_TAC>>
-  fs[dividesTheory.divides_def]
+  fs[dividesTheory.divides_def,NULL_LENGTH,GSYM LENGTH_NON_NIL]
   >-(
-    fs[listTheory.NULL_LENGTH]>>(* to revise; start *)
-    fs[GSYM listTheory.LENGTH_NON_NIL]>>
     ‘512 ≤ LENGTH bits’ by simp[]>>
-    drule_then assume_tac listTheory.LENGTH_TAKE>>
-    ‘LENGTH $ TAKE 512 bits = 32 * 16’ by simp[]>>(* to revise; end *)
+    drule_then assume_tac LENGTH_TAKE>>
+    ‘LENGTH $ TAKE 512 bits = 32 * 16’ by simp[]>>
     drule parse_block_size>>
-    simp[]
-  )
-  >-(
-    fs[listTheory.NULL_LENGTH]>>
-    fs[GSYM listTheory.LENGTH_NON_NIL]>>
-    intLib.ARITH_TAC)
+    simp[])
+  >-intLib.ARITH_TAC
 QED
 
 Theorem parse_message_block_size:
@@ -162,11 +172,6 @@ Proof
   drule_then assume_tac parse_message_size>>
   simp[]
 QED
-
-(*** END ***)
-
-
-
 
 (* dummy final else-branch added to make f well-defined in all cases *)
 Definition f_def:
@@ -253,7 +258,7 @@ QED
 Theorem rho_eq_rho_alt_lt_16:
   n < 16 ⇒ rho n = rho_alt n
 Proof
-  rw[rho_def, rho_alt_def]
+  rw[rho_def,rho_alt_def]
 QED
 
 Triviality suc_help = CONV_RULE numLib.SUC_TO_NUMERAL_DEFN_CONV prim_recTheory.LESS_THM;
@@ -262,29 +267,23 @@ Theorem rho_preserves_lt_16:
   n < 16 ⇒ rho n < 16
 Proof
   rw[rho_def]>>
-  pop_assum (
-    fn thm => (
-      strip_assume_tac (
-        SRULE
-          [suc_help] thm)))>>
+  pop_assum (fn thm => strip_assume_tac $ SRULE [suc_help] thm)>>
   fs[]
 QED
 
 Theorem funpow_rho_preserves_lt_16:
   ∀n m. m < 16 ⇒ FUNPOW rho n m < 16
 Proof
-  Induct
-  >-simp[]
-  >-(
-    rw[FUNPOW]>>
-    last_x_assum irule>>
-    simp[rho_preserves_lt_16])
+  Induct>>
+  rw[FUNPOW]>>
+  last_x_assum irule>>
+  simp[rho_preserves_lt_16]
 QED
 
 Theorem rho_eq_rho_alt_lt_16_funpow:
   m < 16 ⇒ FUNPOW rho n m = FUNPOW rho_alt n m
 Proof
-  rw[]>>
+  strip_tac>>
   irule FUNPOW_CONG>>
   rw[]>>
   irule rho_eq_rho_alt_lt_16>>
@@ -314,8 +313,7 @@ Theorem r_alt_cv:
   in
     FUNPOW rho_alt qt rm
 Proof
-  simp[r_def, rho_def, rho_alt_def]>>
-  rw[rho_eq_rho_alt_lt_16_funpow]
+  rw[r_def,rho_def,rho_alt_def,rho_eq_rho_alt_lt_16_funpow]
 QED
 
 val () = cv_auto_trans r_alt_cv;
@@ -345,8 +343,7 @@ Theorem r'_alt_cv:
   in
     FUNPOW rho_alt qt rm
 Proof
-  simp[r'_def, rho_def, rho_alt_def, pi_def]>>
-  rw[rho_eq_rho_alt_lt_16_funpow]
+  rw[r'_def,rho_def,rho_alt_def,pi_def,rho_eq_rho_alt_lt_16_funpow]
 QED
 
 val () = cv_auto_trans r'_alt_cv;
@@ -354,7 +351,7 @@ val () = cv_auto_trans r'_alt_cv;
 Theorem r'_lt_16:
   r' j < 16
 Proof
-  simp[r'_def, pi_def]>>
+  simp[r'_def,pi_def]>>
   irule funpow_rho_preserves_lt_16>>
   intLib.ARITH_TAC
 QED
@@ -392,11 +389,7 @@ Proof
   >-intLib.ARITH_TAC
   >-intLib.ARITH_TAC
   >-(
-    last_x_assum (
-      fn thm => (
-        strip_assume_tac (
-          SRULE
-          [suc_help] thm)))>>
+    last_x_assum (fn thm => strip_assume_tac $ SRULE [suc_help] thm)>>
     simp[]>>
     EVAL_TAC)
 QED
@@ -423,46 +416,43 @@ Proof
   >-intLib.ARITH_TAC
   >-intLib.ARITH_TAC
   >-(
-    last_x_assum (
-      fn thm => (
-        strip_assume_tac (
-          SRULE
-          [suc_help] thm)))>>
+    last_x_assum (fn thm => strip_assume_tac $ SRULE [suc_help] thm)>>
     simp[]>>
     EVAL_TAC)
 QED
 
 Definition initial_value_def:
-  initial_value: word32 # word32 # word32 # word32 # word32 = (0x67452301w, 0xEFCDAB89w, 0x98BADCFEw, 0x10325476w, 0xC3D2E1F0w)
+  initial_value: word32 # word32 # word32 # word32 # word32 =
+  (0x67452301w,0xEFCDAB89w,0x98BADCFEw,0x10325476w,0xC3D2E1F0w)
 End
 
 val () = cv_trans_deep_embedding EVAL initial_value_def;
 
 Definition rol_def:
-  rol n (x: 'a word) = (x << n) || (x >>> (dimindex(:'a) - n))
+  rol n x: 'a word = (x << n) || (x >>> (dimindex(:'a) - n))
 End
 
 val () = cv_auto_trans (INST_TYPE[alpha |-> ``:32``] rol_def);
 
 Definition inner_for_loop_def:
-  inner_for_loop block (j, (A, B, C, D, E), (A', B', C', D', E')) =
+  inner_for_loop block (j,(A,B,C,D,E),(A',B',C',D',E')) =
   let
     T1 = rol (s  j) (A  + f j        B  C  D  + EL (r  j) block + K  j) + E;
     T2 = rol (s' j) (A' + f (79 - j) B' C' D' + EL (r' j) block + K' j) + E'
   in
-    (SUC j, (E, T1, B, rol 10 C, D), (E', T2, B', rol 10 C', D'))
+    (SUC j,(E,T1,B,rol 10 C,D),(E',T2,B',rol 10 C',D'))
 End
 
 Definition inner_for_loop_alt_def:
-  inner_for_loop_alt block (j, (A, B, C, D, E), (A', B', C', D', E')) =
+  inner_for_loop_alt block (j,(A,B,C,D,E),(A',B',C',D',E')) =
   if j < 80 ∧ LENGTH block = 16 then
     let
       T1 = rol (s  j) (A  + f j        B  C  D  + EL (r  j) block + K  j) + E;
       T2 = rol (s' j) (A' + f (79 - j) B' C' D' + EL (r' j) block + K' j) + E'
     in
-      (SUC j, (E, T1, B, rol 10 C, D), (E', T2, B', rol 10 C', D'))
+      (SUC j,(E,T1,B,rol 10 C,D),(E',T2,B',rol 10 C',D'))
   else
-    (0, (0w, 0w, 0w, 0w, 0w), (0w, 0w, 0w, 0w, 0w))
+    (0,(0w,0w,0w,0w,0w),(0w,0w,0w,0w,0w))
 End
 
 val inner_for_loop_alt_pre_def = cv_trans_pre inner_for_loop_alt_def;
@@ -471,36 +461,36 @@ Theorem inner_for_loop_alt_pre[cv_pre]:
   inner_for_loop_alt_pre block v
 Proof
   simp[inner_for_loop_alt_pre_def]>>
-  rw[r_lt_16, r'_lt_16]
+  rw[r_lt_16,r'_lt_16]
 QED
 
 Theorem inner_for_loop_eq_alt:
   j < 80 ∧ LENGTH block = 16 ⇒
-  inner_for_loop block (j, v) = inner_for_loop_alt block (j, v)
+  inner_for_loop block (j,v) = inner_for_loop_alt block (j,v)
 Proof
   PairCases_on ‘v’>>
-  rw[inner_for_loop_def, inner_for_loop_alt_def]
+  rw[inner_for_loop_def,inner_for_loop_alt_def]
 QED
 
 (* the body of the outer for-loop *)
 Definition process_block_def:
-  process_block (h0, h1, h2, h3, h4) block =
+  process_block (h0,h1,h2,h3,h4) block =
   let
-    hs = FUNPOW (inner_for_loop block) 80 (0, (h0, h1, h2, h3, h4), (h0, h1, h2, h3, h4))
+    hs = FUNPOW (inner_for_loop block) 80 (0,(h0,h1,h2,h3,h4),(h0,h1,h2,h3,h4))
   in
     case hs of
-      (_, (A, B, C, D, E), (A', B', C', D', E')) =>
-        (h1 + C + D', h2 + D + E', h3 + E + A', h4 + A + B', h0 + B + C')
+      (_,(A,B,C,D,E),(A',B',C',D',E')) =>
+        (h1 + C + D',h2 + D + E',h3 + E + A',h4 + A + B',h0 + B + C')
 End
 
 Definition process_block_alt_def:
-  process_block_alt (h0, h1, h2, h3, h4) block =
+  process_block_alt (h0,h1,h2,h3,h4) block =
   let
-    hs = FUNPOW (inner_for_loop_alt block) 80 (0, (h0, h1, h2, h3, h4), (h0, h1, h2, h3, h4))
+    hs = FUNPOW (inner_for_loop_alt block) 80 (0,(h0,h1,h2,h3,h4),(h0,h1,h2,h3,h4))
   in
     case hs of
-      (_, (A, B, C, D, E), (A', B', C', D', E')) =>
-        (h1 + C + D', h2 + D + E', h3 + E + A', h4 + A + B', h0 + B + C')
+      (_,(A,B,C,D,E),(A',B',C',D',E')) =>
+        (h1 + C + D',h2 + D + E',h3 + E + A',h4 + A + B',h0 + B + C')
 End
 
 val () = cv_auto_trans process_block_alt_def;
@@ -520,7 +510,7 @@ Theorem process_block_eq_alt:
   LENGTH block = 16 ⇒ process_block v block = process_block_alt v block
 Proof
   PairCases_on ‘v’>>
-  rw[process_block_def, process_block_alt_def, inner_for_loop_eq_alt]>>
+  rw[process_block_def,process_block_alt_def,inner_for_loop_eq_alt]>>
   AP_THM_TAC>>
   AP_TERM_TAC>>
   irule FUNPOW_CONG>>
@@ -547,7 +537,7 @@ Theorem outer_for_loop_alt_cv:
   EVERY (λe. LENGTH e = 16) blocks ⇒
   outer_for_loop blocks = outer_for_loop_alt blocks
 Proof
-  rw[outer_for_loop_def, outer_for_loop_alt_def]>>
+  rw[outer_for_loop_def,outer_for_loop_alt_def]>>
   irule FOLDL_CONG>>
   rw[]>>
   imp_res_tac EVERY_MEM>>
@@ -566,14 +556,13 @@ val () = cv_auto_trans word32_chg_end_def;
 (* dummy value added for length of input message m exceeding 2 ** 64 *)
 Definition RIPEMD_160_def:
   RIPEMD_160 m: 160 word =
-  if LENGTH m < 2 ** 64
-  then
+  if LENGTH m < 2 ** 64 then
     let
       p      = pad_message m;
       blocks = parse_message [] p
     in
       case outer_for_loop blocks of
-        (h0, h1, h2, h3, h4) =>
+        (h0,h1,h2,h3,h4) =>
           concat_word_list [
             (word32_chg_end h4);
             (word32_chg_end h3);
@@ -585,14 +574,13 @@ End
 
 Theorem RIPEMD_160_alt_cv:
   RIPEMD_160 m =
-  if LENGTH m < 2 ** 64
-  then
+  if LENGTH m < 2 ** 64 then
     let
       p      = pad_message m;
       blocks = parse_message [] p
     in
       case outer_for_loop_alt blocks of
-        (h0, h1, h2, h3, h4) =>
+        (h0,h1,h2,h3,h4) =>
           concat_word_list [
             (word32_chg_end h4);
             (word32_chg_end h3);
@@ -620,7 +608,7 @@ Definition RIPEMD_160_alt_def:
       blocks = parse_message [] p
     in
       case outer_for_loop_alt blocks of
-        (h0, h1, h2, h3, h4) =>
+        (h0,h1,h2,h3,h4) =>
           concat_word_list [
             (word32_chg_end h4);
             (word32_chg_end h3);
@@ -634,7 +622,7 @@ Theorem RIPEMD_160_eq_alt:
   LENGTH m < 2 ** 64 ⇒ RIPEMD_160 m = RIPEMD_160_alt m
 Proof
   strip_tac>>
-  simp[RIPEMD_160_def, RIPEMD_160_alt_def]>>
+  simp[RIPEMD_160_def,RIPEMD_160_alt_def]>>
   drule_then assume_tac parse_message_block_size>>
   drule_then assume_tac outer_for_loop_alt_cv>>
   rw[]
